\section{The modular group}

Throughout this section and also later, we adopt the notation of Schoeneberg \cite{schoeneberg1974elliptic}.

\begin{definition}
\label{dfn_ModularGroup}
\index{Modular!group}
\index{Modular!transformation}
\index{Inhomogeneous!modular transformation}
A Möbius transformation $\phi$ of the form
\begin{equation*}
\phi(z) = \moebius{a}{b}{c}{d}{z},\quad a,b,c,d \in \Z,\quad ad - bc = 1
\end{equation*}
is called \emph{(inhomogeneous) modular transformation}.
\end{definition}

\begin{theorem}
\label{thm_ModularGroup}
\index{Modular!group}
The set of modular transformations forms a discrete subgroup of the group of Möbius transformations and can be identified with the projective special linear group $\PSL{\Z}$. This group is called the \emph{modular group} and is denoted by $\ModGrp$.
\end{theorem}
\begin{proof}
The proof is very similar to that of Theorem \ref{thm_MoebiusGroup}. The only thing which has to be changed is the homomorphism $\pi$ defined in (\ref{eqn_homPi}). Its domain now is $\SL{\Z}$, the group of 2-by-2 matrices over $\Z$ with determinant 1, rather than $\GL{\C}$ (or $\SL{\C}$). Again it follows by the first isomorphism theorem, that the modular group $\ModGrp$ is isomorphic to $\SL{\Z} / \ker(\pi) \cong \PSL{\Z}$. The fact that $\ModGrp$ is a discrete subgroup of the group of Möbius transformations is now also directly evident.
\end{proof}

\begin{remark}
\index{Inhomogeneous!modular transformation}
\index{Homogeneous!modular transformation}
\index{Modular!transformation}
The elements of $\SL{\Z}$ are often called \emph{homogeneous modular transformations}, whereas the transformations of $\ModGrp = \PSL{\Z}$ are called \emph{inhomogeneous transformations}. Strictly seen, an inhomogeneous transformation has to be denoted as $[M]_{\sim}$, which is the equivalence class in $\PSL{\Z}$ of a matrix $M \in \SL{\Z}$. It is clear, that $[M]_{\sim}$ is nothing but the set $\{\pm M\}$ and again for easier notation, we will from now on simply write either $M$ or $-M$ instead of $[M]_{\sim}$. Additionally we will denote equivalence of matrices by $\sim$, \ie, if $\lambda = \pm 1$, then $M \sim \lambda M$.
\end{remark}

\todo{16}{Basic mapping properties}

\subsection{Generators and relations}

In group theory it is an important question, which systems of group elements and relations completely describe the structure of any given group (in the sense of definition \ref{dfn_GrpConstructGenRel}). This section is devoted to the investigation of this question in the case of the modular group.

Before we start, we introduce the following three important modular transformations which will be used very frequently from now on:

\begin{IEEEeqnarray*}{RL}
U: & z \mapsto z + 1 \\
T: & z \mapsto -\reci{z} \\
R = TU: & z \mapsto -\reci{z + 1}
\end{IEEEeqnarray*}

\begin{remark}
Unfortunately, in literature there is no consensus on the notation of these transformations. We use the notation of Schoeneberg \cite{schoeneberg1974elliptic} here, but other notations are frequent. For example in Klein/Fricke \cite{klein1966vorlesungen}, the symbol $S$ is used instead of $U$ and in other literature as well as on Wikipedia, additionally the roles of $S$ and $T$ are swapped.
\end{remark}

\begin{theorem}
\label{thm_ModGrpGen}
The modular group is generated by the elements $U: z \mapsto z+1$ and $T: z \mapsto -\reci{z}$. 
\end{theorem}
\begin{proof}
Let $A: z \mapsto \moebius{a}{b}{c}{d}{z}$ be an arbitrary modular transformation. Our goal is to show that $A$ can be written as product of the transformations $U$ and $T$. For this purpose it is more convenient to view these transformations as elements of $\PSL{\Z}$, namely
\begin{equation*}
A = \mat{a}{b}{c}{d}, \quad U = \mat{1}{1}{0}{1}, \quad T = \mat{0}{-1}{1}{\phantom{+}0}.
\end{equation*}

Let's first consider the two special cases, when $a$ or $c$ are zero. If $a=0$, it follows from $ad - bc = 1$, that $-b = c = \pm 1$. Therefore we have (equivalence of Matrices is again denoted by $\sim$)
\begin{equation*}
A \sim c A = \mat{0}{-1}{1}{c d} = TU^{c d}.
\end{equation*}
Similarly, $c = 0$ gives $a = d = \pm 1$ and
\begin{equation*}
A \sim a A = \mat{1}{a b}{0}{1} = U^{a b}.
\end{equation*}
In the general case, when $a$ and $c$ are both nonzero, $ad - bc = 1$ implies that $a$ and $c$ are coprime and the Euclidean algorithm therefore yields
\begin{eqnarray*}
      a &=& q_0 \cdot c\phantom{_0} + r_1 \\
      c &=& q_1 \cdot r_1 + r_2 \\
    r_1 &=& q_2 \cdot r_2 + r_3 \\
        &\vdots& \\
r_{n-1} &=& q_n \cdot r_n + r_{n+1}\\
        &=& q_n \cdot 1\phantom{_n} + 0.
\end{eqnarray*}
We can use this to reduce the Matrix $A$ by successively multiplying powers of $U$ and $T$ from the left. Just note, that multiplication with $U^k$ adds $k$ times the second row to the first row, whereas $T$ swaps the rows and changes the sign of one arbitrary row\footnote{This freedom of choice is again due to the fact that the matrices $M$ and $-M$ represent the same element in $\PSL{\Z}$.}. If we concentrate only on the first column of $A$ and apply the first few transformations
\begin{equation*}
\cvec{a}{c}                           \overset{U^{-q_0}}{\longmapsto}
\cvec{r_1}{c\phantom{_1}}             \overset{T}{\mapsto} 
\cvec{\phantom{+}c\phantom{_1}}{-r_1} \overset{U^{q_1}}{\longmapsto}
\cvec{\phantom{+}r_2}{-r_1}           \overset{T}{\mapsto} 
\cvec{r_1}{r_2}                       \overset{U^{-q_2}}{\longmapsto}
\cvec{r_3}{r_2}                       \overset{T}{\mapsto}
\cvec{\phantom{+}r_2}{-r_3}           \mapsto \dots,
\end{equation*}
we soon recognize the general mapping rule, which is
\begin{IEEEeqnarray*}{rCll}
\cvec{\phantom{+}r_{j-1}}{\phantom{+}r_{j\phantom{+0}}} 
& \overset{TU^{-q_j}}{\longmapsto}
& \cvec{\phantom{+}r_{j\phantom{+0}}}{-r_{j+1}}
& \quad \text{for even } j \text{ and}\\
\cvec{\phantom{+}r_{j-1}}{-r_{j\phantom{+0}}}
& \overset{TU^{q_j}}{\longmapsto}
& \cvec{\phantom{+}r_{j\phantom{+0}}}{\phantom{+}r_{j+1}} 
& \quad \text{for odd } j.
\end{IEEEeqnarray*}
When we set $r_{-1} := a$ and $r_0 := c$, this rule is true for $0 \le j \le n$. Obviously the described procedure ends with
\begin{equation*}
\cdots \overset{T}{\mapsto}
\cvec{\phantom{+}r_{n\phantom{+0}}}{\pm r_{n+1}} = \cvec{1}{0}.
\end{equation*} 
Because we know the first column of the resulting matrix and its determinant, which is 1, we can conclude that for some $k \in \Z$ it must have the form
\begin{equation*}
\mat{1}{k}{0}{1} = U^k.
\end{equation*}
By setting $e_n := (-1)^{n} q_n$, we therefore have 
\begin{equation*}
TU^{-e_n} TU^{-e_{n-1}} \cdots TU^{-e_1}TU^{-e_0} A = U^k
\end{equation*}
or equivalently,
\begin{equation*}
A = U^{e_0} TU^{e_1} \cdots TU^{e_{n-1}} TU^{e_n} T U^k,
\end{equation*}
which gives the desired representation of $A$ in terms of $U$ and $T$ in the case when $a$ and $c$ are both non-zero.
\end{proof}

It is worth formulating the algorithm used in the previous proof explicitly in the following corollary.
\begin{corollary}
\label{cor_ModGrpTUAlg}
An arbitrary modular transformation $A: z \mapsto \moebius{a}{b}{c}{d}{z}$ can be represented in terms of the transformations $U: z \mapsto z+1$ and $T : z \mapsto -\reci{z}$, by performing the following steps:
\begin{enumerate}
\item If $a = 0$, then $A = TU^{c d}$ and if $c = 0$, then $A = U^{a b}$ and we are done. Otherwise, continue with \ref{itm_ModGrpTUAlgStart}.
\item \label{itm_ModGrpTUAlgStart} Apply the Euclidean algorithm to $a$ and $c$ with the first division being $a = q_0 \cdot c + r_1$ ($q_0$ may be $\le 0$) and let $n$ be the number of the  last division (start counting from 0). Call the arising quotients $q_0,q_1,\dots,q_n$.
\item For $j \in \{0,1,\dots,n\}$ set $e_j := (-1)^j q_j$.
\item Calculate the matrix product $TU^{-e_n} TU^{-e_{n-1}} \cdots TU^{-e_1}TU^{-e_0} A$ and multiply by $\pm 1$ in order to obtain a representation with positive diagonal elements. Read off the right-upper entry and call it $k$.
\end{enumerate}
The transformation $A$ can now be written as
\begin{equation}
\label{eqn_ModGrpTUAlg}
A = U^{e_0} TU^{e_1} \cdots TU^{e_{n-1}} TU^{e_n} T U^k.
\end{equation}
\end{corollary}

We have seen that $T$ and $U$ generate the modular group, but it is not yet clear, which group words in $T$ and $U$ give the same modular transformations. For example, it is easy to see that $T^2 = 1$ and $(TU)^3 = 1$ are relations which are satisfied by $T$ and $U$. It is the goal of the following paragraphs to show that these two relations are in fact the only ones in the sense that all other relations are derived from these. For this purpose we first define the three characteristic properties for modular transformations:

\begin{definition}
For a modular transformation $A: z \mapsto \moebius{a}{b}{c}{d}{z}$ we define the predicates $t$, $r$ and $s$:
\begin{IEEEeqnarray}{rCcCc}
\label{eqn_tpred}
t(A) &:\quad& ac \ge 0       &\quad\land\quad& bd \ge 0 \\
\label{eqn_rpred}
r(A) &:\quad& a^2 + ac \le 0 &\quad\land\quad& b^2 + bd \le 0 \\
\label{eqn_spred}
s(A) &:\quad& c^2 + ac \le 0 &\quad\land\quad& d^2 + bd \le 0
\end{IEEEeqnarray}
\end{definition}

Note, that $t$, $r$ and $s$ are well-defined, since they do not change their value if we switch from the matrix $A \in \PSL{\Z}$ to the equivalent matrix $-A$, \eg $t(A) \Leftrightarrow t(-A)$.

\begin{lemma}
Let $A: z \mapsto \moebius{a}{b}{c}{d}{z}$ be an arbitrary modular transformation. Then one, and only one of the predicates $t(A)$, $r(A)$ and $s(A)$ is true.
\end{lemma}
\begin{proof}
We start by considering the two easiest cases first: If $A$ is the identity transformation or $A = T$, we have $t(A)$, $\lnot r(A)$ and $\lnot s(A)$.

For all other cases, we note that at least three of the coefficients $a,b,c,d$ are nonzero. Therefore, if one of the predicates $t(A), r(A), s(A)$ is satisfied, then at least one of the two inequalities involved is \emph{strictly} fulfilled. Having this said, it is easy to see that $t(A) \Rightarrow \lnot r(A) \land \lnot s(A)$. Thus it remains to show 
\begin{equation*}
\lnot t(A) \Rightarrow r(A) \lxor s(A),
\end{equation*}
for all transformations with at least three nonzero coeffisients (here, $\lxor$ denotes logical exclusive or). If $t(A)$ is false, we have $ac < 0$ or $bd < 0$. Since both cases are completely symmetric, we may assume without restriction that $ac < 0$. Note, that $ac < 0$ and $ad - bc = 1$ implies $bd \le 0$ because otherwise if $bd > 0$, both terms $ad$ and $bc$ would have different signs and their difference could not be 1. We conclude the proof by distinguishing three cases:
\begin{description}
\item[Case $a^2 < c^2$:] From $ac < 0$ it follows that $a^2 + ac < 0\ (i)$ and $c^2 + ac > 0\ (ii)$. Additionally, from $ad - bc = 1$ we can conclude that $b^2 \le d^2$, because otherwise $\abs{ad}$ would differ from $\abs{bc}$ by more than 1. Therefore we also have $b^2 + bd \le 0\ (iii)$. Taking these pieces together, we have $(ii) \Rightarrow \lnot s(A)$ and $(i) \land (iii) \Rightarrow r(A)$.
\item[Case $a^2 > c^2$:] This case is complementary to the first one: Because of $ac < 0$ we have $a^2 + ac > 0\ (i)$ and $c^2 + ac < 0\ (ii)$. The equation $ad - bc = 1$ here implies $b^2 \ge d^2$ and $d^2 + bd \le 0\ (iii)$. Thus we have $(i) \Rightarrow \lnot r(A)$ and $(ii) \land (iii) \Rightarrow s(A)$.
\item[Case $a^2 = c^2$:] Note that this case is only possible with $a = -c = \pm 1$ (as $a$ and $c$ are coprime). Hence we have $a^2 + ac = c^2 + ac = 0$. However, $ad - bc = 1$ implies $b^2 \ne d^2$ and therefore we have $b^2 + bd \le 0 \lxor d^2 + bd \le 0$. So, also in this case we have $r(A) \lxor s(A)$.\qedhere
\end{description}
\end{proof}

\begin{theorem}
\label{thm_ModGrpRel}
The generators $T: z \mapsto -\reci{z}$ and $R: z \mapsto -\reci{z+1}$ of the modular group satisfy the relations
\begin{equation}
\label{eqn_ModGrpTRRel}
T^2 = \id{\C}, \quad R^3 = \id{\C}
\end{equation}
and all other relations are derived from these two. Therefore the modular group is isomorphic to the free product of a cyclic group of order 2 and a cyclic group of order 3.
\end{theorem}

\todo{18}{Proof}

% ------------------------------- Subsection: Fundamental domains, tessellation
\input{sub-fundomtess.tex}

% --------------------------------------------- Subsection: Hyperbolic geometry
\input{sub-hypgeom.tex}

% ------------------------------- Subsection: Ford circles, continued fractions
\input{sub-fordconf.tex}

